fill in more proof

src/examples/implang_cont_eg.v
@@ -26,9 +26,26 @@ Section spec.
   Context `{!gen_heapGS loc val Σ} `{!envGS val Σ} `{!invGS_gen HasNoLc Σ}.
 
   Local Open Scope bi_scope.
+  Local Open Scope Z_scope.
 
   Definition min_positive_r (lv: list Z) : Z :=
-    foldr Z.min 0%Z lv.
+    Z.max 0 (foldr Z.min 0 lv).
+
+  Lemma min_positive_r_cons x l : min_positive_r (x::l) = Z.max 0 (Z.min x (min_positive_r l)).
+  Proof.
+    rewrite /min_positive_r /=. lia.
+  Qed.
+
+  Lemma min_positive_r_app_r (lv_a : list Z) (z: Z) :
+    z ≤ 0 →
+    min_positive_r (lv_a ++ [z]) = min_positive_r lv_a.
+  Proof.
+    revert z.
+    induction lv_a as [|x lv_a IH]; intros.
+    - rewrite /min_positive_r /=; lia.
+    - rewrite -app_comm_cons min_positive_r_cons IH //.
+      rewrite /min_positive_r /=. lia.
+  Qed.
 
   Definition ptr_add (l: loc) (i: Z) : loc :=
     (l + i)%Z.
@@ -57,7 +74,19 @@ Section spec.
 
   Notation "l ↦ₛ lv" := (llist_seg l lv) (at level 9) : bi_scope.
   Notation "l ↦ₗ lv" := (llist l lv) (at level 10) : bi_scope.
-
+  
+  Lemma llist_seg_app l lv1 lv2 last :
+    l ↦ₛ (lv1 ++ lv2) last ⊣⊢ ∃ l', l ↦ₛ lv1 l' ∗ l' ↦ₛ lv2 last.
+  Proof.
+    revert l.
+    induction lv1 => ?; simpl.
+    - iSplit; by [iIntros "$"|iIntros "(% & -> & $)"].
+    - iSplit; iIntros "H".
+      + iDestruct "H" as "(% & %l' & $ & $ & H3)". rewrite IHlv1.
+        by iDestruct "H3" as "(% & $ & $)".
+      + iDestruct "H" as "(% & (% & % & $ & $ & H2) & H3)".
+        iSplit; first done. rewrite IHlv1. iFrame.
+  Qed.
 
   (* FIXME make this into a lemma up1_fupd *)
   (* equiv to rewrite /= !(monPred_at_fupd(BiFUpd0:=uPred_bi_fupd)). *)
@@ -68,7 +97,7 @@ Section spec.
     end.
 
   (* ad-hoc, aggressive *)
-  Ltac iSteps := repeat first [iStep | iModIntro | progress iFrame | progress iIntros ].
+  Ltac iSteps := repeat first [iStep | iModIntro | progress iFrame | progress iIntros | progress simpl].
 
   Lemma min_positive_spec E (l: loc) (lv: list Z) :
     (∃ _z, "r" ↦v NumV _z) ∗ l ↦ₗ lv
@@ -77,15 +106,13 @@ Section spec.
     iIntros "((%_z & r) & arr)".
     wp_start_func with_retainer "retainer" and_locals "(l & min & v & _)".
     iSteps.
-    simpl.
-
     set (∃ l_m lv_a lv_b v,
           (* split arr into two parts *)
           ⌜lv = lv_a++lv_b ⌝ ∧ l ↦ₛ lv_a l_m ∗ l_m ↦ₗ lv_b ∗ 
           (* "min" always store min of the first part*)
           "l" ↦v (LocV l_m) ∗ "v" ↦v v ∗ "min" ↦v (NumV (min_positive_r lv_a)) ∗
           stack_retainer min_positive ∗ (∃ _z, ⇓ ("r" ↦v _z)))%I%Z as inv.
-    wp_apply (wp_while_inv  _ _ _ _ inv with "[] [-]" ) ; simpl.
+    wp_apply (wp_while_inv  _ _ _ _ inv with "[] [-]" ); simpl.
     {
       iIntros "!> (%l_m & %lv_a & %lv_b & %v & -> & arr_a & arr_b & l & v & min & retainer & (%_z' & r))".
       iSteps.
@@ -96,12 +123,29 @@ Section spec.
         iSplitL "l v min".
         { iExists [_;_;_]. iSplit; first done. by iFrame. }
         iIntros "!> !> r". iFrame.
-        destruct lv_b. 2: { rewrite /llist {2}/llist_seg /=. iDestruct "arr_b" as "[% ?]". done. }
+        destruct lv_b. 2: { iDestruct "arr_b" as "[% ?]". done. }
         rewrite app_nil_r. iFrame.
       - iExists _. iSplit; first done.
-        iSteps. simpl.
         iSteps.
-        admit.
+        destruct lv_b. { iDestruct "arr_b" as "%". done. }
+        iDestruct "arr_b" as "(% & %l_n & arr_b_0 & arr_b_1 & arr_c)". fold llist_seg.
+        iFrame. iIntros "arr_b_0".
+        iFrame. iIntros "!> v".
+        iSteps.
+        destruct (bool_decide (z ≤ 0)%Z) eqn:Heqz;
+          [rewrite bool_decide_eq_true in Heqz; subst | rewrite bool_decide_eq_false in Heqz].
+        + iExists _. iSplit; first done.
+          iModIntro. simpl. iStep. simpl.
+          iRename select (⎡pointsto (l_m + 1)%Z _ _⎤)%I into "arr_b_1".
+          iPoseProof (bi.equiv_entails_1_2  _ _ (llist_seg_app l lv_a [z] l_n) with "[$arr_a $arr_b_0 $arr_b_1]") as "?".
+          { done. }
+          iFrame.
+          rewrite -app_assoc /= min_positive_r_app_r //.
+          by iFrame.
+        + iExists _. iSplit; first done.
+          iSteps.
+          (* FIXME fill in the boring case analysis here *)
+          admit.
     }
     {
       rewrite /inv. iFrame. iExists []. rewrite app_nil_l /=. by iFrame.
@@ -109,8 +153,15 @@ Section spec.
     iSteps.
     iRename select (_) into "inv".
     iDestruct "inv" as "(%l_m & %lv_a & %lv_b & %v & -> & arr_a & arr_b & l & v & min & retainer & (%_z' & r))".
-    (* TODO need to show that it has traversed through the whole list, i.e. l_m=0 or lv_b=[] *)
     iSteps.
+    rewrite /BoolV in H.
+    destruct (bool_decide (l_m = 0%Z)) eqn:Heqb; rewrite Heqb in H;
+      [rewrite bool_decide_eq_true in Heqb; subst | done].
+    iSplitL "l v min".
+    { iExists [_;_;_]. iSplit; first done. by iFrame. }
+    iIntros "!> !> r". iFrame.
+    destruct lv_b. 2: { rewrite /llist {2}/llist_seg /=. iDestruct "arr_b" as "[% ?]". done. }
+    rewrite app_nil_r. iFrame.
   Admitted.
 
 End spec.
